

التقييم الأسبوعي الرابع بصفة

1 / 1

المجموعة الأولى

$$[1] \quad 0 = (1-1) + (1-1) + (1-1)$$

$$= 0 - 1 - 1 = -2$$

$$= (1-1)$$

الدالة فردية

[2] تنازلية في $[-\infty, 0]$

تناقصية في $[0, \infty]$

$$[3] \quad \frac{f(4) - f(2)}{4 - 2} = \frac{17 - 11}{4 - 2} = \frac{6}{2} = 3$$

كمية في كمية

$$1 = \frac{1}{1} = \frac{(1-1)}{(1-1)}$$

$$[4] \quad \frac{f(4) - f(2)}{4 - 2} = \frac{17 - 11}{4 - 2} = \frac{6}{2} = 3$$

كمية في كمية

$$[5] \quad \frac{f(4) - f(2)}{4 - 2} = \frac{17 - 11}{4 - 2} = \frac{6}{2} = 3$$

$$[6] \quad \frac{f(4) - f(2)}{4 - 2} = \frac{17 - 11}{4 - 2} = \frac{6}{2} = 3$$

$$\frac{1 + \sqrt{1-1}}{1 + \sqrt{1-1}} \times \frac{1-1}{1-1} = \frac{1-1}{1-1} = 0$$

$$[7] \quad \frac{f(4) - f(2)}{4 - 2} = \frac{17 - 11}{4 - 2} = \frac{6}{2} = 3$$

المجموعة الثانية

$$[1] \quad 0 = (1-1) + (1-1) + (1-1)$$

$$= 0 - 1 - 1 = -2$$

الدالة زوجية

[2] تنازلية في $[-\infty, 0]$

$$[3] \quad \frac{f(4) - f(2)}{4 - 2} = \frac{17 - 11}{4 - 2} = \frac{6}{2} = 3$$

$$1 = \frac{1}{1} = \frac{(1-1)}{(1-1)}$$

$$[4] \quad \frac{f(4) - f(2)}{4 - 2} = \frac{17 - 11}{4 - 2} = \frac{6}{2} = 3$$

$$[5] \quad \frac{f(4) - f(2)}{4 - 2} = \frac{17 - 11}{4 - 2} = \frac{6}{2} = 3$$

$$[6] \quad \frac{f(4) - f(2)}{4 - 2} = \frac{17 - 11}{4 - 2} = \frac{6}{2} = 3$$

$$\frac{1 + \sqrt{1-1}}{1 + \sqrt{1-1}} \times \frac{1-1}{1-1} = \frac{1-1}{1-1} = 0$$

$$[7] \quad \frac{f(4) - f(2)}{4 - 2} = \frac{17 - 11}{4 - 2} = \frac{6}{2} = 3$$

المبحث ١٠ - الدالة التفاضلية

$$\begin{aligned} \text{د (١)} &= (١-٣) + (٣-١) = ٢ \\ (٣-١) - (١-٣) &= ٢ - ٢ = ٠ \\ \text{د (٢)} &= \text{الدالة غير موجودة} \end{aligned}$$

$$\begin{aligned} \text{تناقصية في } [٢, ٤] \\ \text{تزايدية في } [٤, ٦] \end{aligned}$$

$$\begin{aligned} \text{د (٦)} &= \frac{\text{مشتق}}{٦-٣-٣} = \frac{\text{مشتق}}{\text{مشتق}} \\ \text{نما} &= \frac{(٦-٣)}{(١+٣)(٦-٣)} = \frac{١}{٤} \end{aligned}$$

$$\begin{aligned} \text{د (٥)} &= \frac{٥-٥}{٥-٥} = \frac{\text{مشتق}}{\text{مشتق}} \\ \text{نما} &= \frac{(٥+٣)(٥-٣)}{(٥-٣)} = ١٠ \end{aligned}$$

$$\text{د (٢)} = \frac{\text{مشتق}}{٣-٣} = \frac{\text{مشتق}}{\text{مشتق}}$$

$$\text{نما} = \frac{٣-٣}{٣-٣+\sqrt{٣-٣}} = \frac{٠}{٠}$$

$$\text{نما} = \frac{(٣+\sqrt{٣-٣})(٣-٣)}{(٣-٣)(٣+\sqrt{٣-٣})} = ١$$